WIP

code/ecdsa/Hacl.Impl.P384.Exponent.fst
@@ -15,100 +15,292 @@ open Spec.ECC.Curves
 open Hacl.Impl.EC.MontgomeryMultiplication
 open Hacl.Impl.EC.LowLevel
 
+open FStar.Math.Lemmas
+open Hacl.Lemmas.P256
+
+open FStar.Tactics 
+open FStar.Tactics.Canon 
+
+open Hacl.Spec.MontgomeryMultiplication
+
+
 #set-options "--z3rlimit 100 --ifuel 0 --fuel 0"
 
+let fromDomain_ = fromDomain_ #P384 #DH
+let toDomain_ = toDomain_ #P384 #DH
 
-[@ CInline]
-val exponent_p384: a: felem P384 -> result: felem P384 -> 
-  tempBuffer: lbuffer uint64 (getCoordinateLenU P384 *. 8ul) -> Stack unit
-  (requires fun h -> live h a /\ live h tempBuffer /\ live h result /\ disjoint tempBuffer result /\ 
-    disjoint a tempBuffer /\ as_nat P384 h a < prime256)
-  (ensures fun h0 _ h1 -> modifies2 result tempBuffer h0 h1 /\ (
-    let k = fromDomain #P384 (as_nat P384 h0 a) in 
-    as_nat P384 h1 result =  toDomain #P384 (pow k (prime384 - 2) % prime256)))
+let as_nat h1 result = as_nat P384 h1 result
+
+val lemma_mod_mul_distr: a: nat -> b: nat -> prime: pos -> Lemma 
+  ((a % prime * (b % prime)) % prime ==  a * b % prime)
+
+let lemma_mod_mul_distr a b prime = 
+  lemma_mod_mul_distr_l a (b % prime) prime;
+  lemma_mod_mul_distr_r a b prime
 
 
-let exponent_p384 t result tempBuffer = 
-  let h0 = ST.get () in 
+val lemma_mod_mul_distr1: a: nat -> b: nat -> c: nat -> prime: pos -> Lemma
+  ((pow a b % prime) * (pow a c % prime) % prime == pow a (b + c) % prime)
 
-  let t0 = sub tempBuffer (size 0) (size 6) in 
+let lemma_mod_mul_distr1 a b c prime = 
+  lemma_mod_mul_distr (pow a b) (pow a c) prime;
+  pow_plus a b c
 
-  let t1 = sub tempBuffer (size 6) (size 6) in 
-  let t2 = sub tempBuffer (size 12) (size 6) in 
-  let t3 = sub tempBuffer (size 18) (size 6) in 
-  let t4 = sub tempBuffer (size 24) (size 6) in 
-  let t5 = sub tempBuffer (size 30) (size 6) in (* 
-  let t6 = sub tempBuffer (size 24) (size 4) in 
-  let t7 = sub tempBuffer (size 28) (size 4) in 
- *)
 
+val exponent0: t: felem P384 -> t0: felem P384 -> t1: felem P384 -> t2: felem P384 -> t3: felem P384 ->  Stack unit 
+  (requires fun h -> live h t /\ live h t0 /\ live h t1 /\ live h t2 /\ live h t3 /\
+    LowStar.Monotonic.Buffer.all_disjoint [loc t; loc t0; loc t1; loc t2; loc t3] /\
+    as_nat h t < prime384)
+  (ensures fun h0 _ h1 -> modifies (loc t0 |+| loc t1 |+| loc t2 |+| loc t3) h0 h1 /\
+    as_nat h1 t < prime384 /\ as_nat h1 t0 < prime384 /\ as_nat h1 t1 < prime384 /\ as_nat h1 t2 < prime384 /\ 
+    as_nat h1 t3 < prime384 /\ (
+    let tD = fromDomain_ (as_nat h0 t) in 
+    as_nat h1 t0 = toDomain_ (pow tD 7 % prime384) /\
+    as_nat h1 t1 = toDomain_ (pow tD 63 % prime384) /\
+    as_nat h1 t2 = toDomain_ (pow tD (126 * pow2 5 + 63) % prime384) /\
+    as_nat h1 t3 = toDomain_ (pow tD (63 * (pow2 7 + 2) *  pow2 11)  % prime384)))
+
+
+let exponent0 t t0 t1 t2 t3 = 
+  let h0 = ST.get() in 
 (* _10     = sq(t) *)
 (* t0 = _10  *)
   montgomery_square_buffer_dh #P384 t t0;
+    let h1 = ST.get() in 
 
 (* _11     = m(t, _10) *)
   montgomery_multiplication_buffer_dh #P384 t t0 t0;
+    let h2 = ST.get() in 
 (* t0 = _11*)
 
 (* _110    = sq(_11) *)
   montgomery_square_buffer_dh #P384 t0 t0;
+    let h3 = ST.get() in 
 (* t0 = _110 *)  
 
 (* _111    = m(t, _110) *)
   montgomery_multiplication_buffer_dh #P384 t t0 t0;
+    let h4 = ST.get() in 
 (* t0 = _111 *)  
 
 (* _111000 (t1) = n_sq(_111, 3) *)
   montgomery_square_buffer_dh #P384 t0 t1;
+    let h5 = ST.get() in 
+    
   fsquarePowN_dh #P384 (size 2) t1;
+    let h6 = ST.get() in 
 (* t1 = sq _111 *)
 (* t1 = n_sq _111 3  *)
 (* t1 = _111000 *)
 
-
 (* _111111 = m(_111,  _111000) *)
   montgomery_multiplication_buffer_dh #P384 t0 t1 t1;  
+    let h7 = ST.get() in 
 (* t1 = t0 * t1 *)
 (* t1 = _111 * _111000 *)
 (* t1 = _111111 *)
 
-
-
 (* x12     = m(n_sq(_111111, 6), _111111) *)
   montgomery_square_buffer_dh #P384 t1 t2;
+    let h8 = ST.get() in 
+
   fsquarePowN_dh #P384 (size 5) t2 ;
+    let h9 = ST.get() in 
   montgomery_multiplication_buffer_dh #P384 t2 t1 t2;
+    let h10 = ST.get() in 
 (* t2 = x12 *)
-
-
-
-(* x24     = m(n_sq(x12 , 12), x12) *)
+  
+  (* x24     = m(n_sq(x12 , 12), x12) *)
   montgomery_square_buffer_dh #P384 t2 t3;
+    let h11 = ST.get() in 
+    
   fsquarePowN_dh #P384 (size 11) t3 ;
-  montgomery_multiplication_buffer_dh #P384 t2 t3 t2;
+    let h12 = ST.get() in 
+    
 (* t2 = x24*) 
 
+  let tD = fromDomain_ (as_nat h0 t) in
+  Hacl.Lemmas.P256.power_one_2 tD;
+  
+  assert(as_nat h1 t0 = toDomain_ (tD * tD % prime384));
+  assert(as_nat h3 t0 = toDomain_ (fromDomain_ (as_nat h2 t0) * fromDomain_ (as_nat h2 t0) % prime384));
+  assert(as_nat h4 t0 = toDomain_ (tD * fromDomain_ (as_nat h3 t0) % prime384));
+  assert(as_nat h5 t1 = toDomain_ (fromDomain_ (as_nat h4 t0) * fromDomain_ (as_nat h4 t0) % prime384));
+  assert(as_nat h6 t1 = toDomain_ (pow (fromDomain_ (as_nat h5 t1)) 4 % prime384));
+  
+  calc (==) {
+    as_nat h2 t0;
+    (==) {}
+    toDomain_ (tD * (pow tD 1 * pow tD 1 % prime384) % prime384);
+    (==) {pow_plus tD 1 1}
+    toDomain_ (tD * (pow tD 2 % prime384) % prime384);
+    (==) {lemma_mod_mul_distr_r tD (pow tD 2) prime384}
+    toDomain_ (pow tD 1 * pow tD 2 % prime384);
+    (==) {pow_plus tD 1 2}
+    toDomain_ (pow tD 3 % prime384);};
+
+  calc (==) {
+    as_nat h3 t0;
+    (==) {}
+    toDomain_ ((pow tD 3 % prime384) * (pow tD 3 % prime384) % prime384); 
+    (==) {lemma_mod_mul_distr_l (pow tD 3) (pow tD 3 % prime384) prime384; 
+      lemma_mod_mul_distr_l (pow tD 3) (pow tD 3) prime384}
+    toDomain_ (pow tD 3 * pow tD 3 % prime384);
+    (==) {pow_plus tD 3 3}
+    toDomain_ (pow tD 6 % prime384);};
+
+  calc (==) {
+    as_nat h4 t0;
+    (==) {}
+    toDomain_ (tD * (pow tD 6 % prime384) % prime384);
+    (==) {lemma_mod_mul_distr_r tD (pow tD 6) prime384}
+    toDomain_ (pow tD 1 * pow tD 6 % prime384);
+    (==) {pow_plus tD 1 6}
+    toDomain_ (pow tD 7 % prime384);};
+
+  calc (==) {
+    as_nat h5 t1;
+    (==) {}
+    toDomain_ (pow tD 7 % prime384 * (pow tD 7 % prime384) % prime384);
+    (==) {lemma_mod_mul_distr (pow tD 7) (pow tD 7) prime384}
+    toDomain_ (pow tD 7 * pow tD 7 % prime384);
+    (==) {pow_plus tD 7 7}
+    toDomain_ (pow tD 14 % prime384); };
+
+  calc (==) {
+    as_nat h6 t1;
+    (==) {}
+    toDomain_ (pow (pow tD 14 % prime384) 4 % prime384);
+    (==) {power_distributivity (pow tD 14) 4 prime384}
+    toDomain_ (pow (pow tD 14) 4 % prime384);
+    (==) {power_mult tD 14 4}
+    toDomain_ (pow tD 56 % prime384); };
+
+  calc (==) {
+    as_nat h7 t1;
+    (==) {}
+    toDomain_ ((pow tD 7 % prime384) * (pow tD 56 % prime384) % prime384);
+    (==) {lemma_mod_mul_distr (pow tD 7) (pow tD 56) prime384}
+    toDomain_ ((pow tD 7) * (pow tD 56) % prime384);
+    (==) {pow_plus tD 7 56}
+    toDomain_ (pow tD 63 % prime384);};
+
+  calc (==) {
+    as_nat h8 t2;
+    (==) {}
+    toDomain_ ((pow tD 63 % prime384) * (pow tD 63 % prime384) % prime384);
+    (==) {lemma_mod_mul_distr1 tD 63 63 prime384}
+    toDomain_ (pow tD 126 % prime384);};
+
+  calc (==) {
+    as_nat h9 t2;
+    (==) {}
+    toDomain_ (pow (pow tD 126 % prime384) (pow2 5) % prime384);
+    (==) {power_distributivity (pow tD 126) (pow2 5) prime384}
+    toDomain_ (pow (pow tD 126) (pow2 5) % prime384);
+    (==) {power_mult tD 126 (pow2 5)}
+    toDomain_ (pow tD (126 * pow2 5) % prime384);};  
+
+  calc (==) {
+    as_nat h10 t2;
+    (==) {}
+    toDomain_ (pow tD (126 * pow2 5) % prime384 * (pow tD 63 % prime384) % prime384);
+    (==) {lemma_mod_mul_distr1 tD (126 * pow2 5) 63 prime384}
+    toDomain_ (pow tD (126 * pow2 5 + 63) % prime384);};
+
+  calc (==) {
+    as_nat h11 t3;
+    (==) {}
+    toDomain_ (pow tD (126 * pow2 5 + 63) % prime384 * (pow tD (126 * pow2 5 + 63) % prime384) % prime384);
+    (==) {lemma_mod_mul_distr1 tD (126 * pow2 5 + 63) (126 * pow2 5 + 63) prime384}
+    toDomain_ (pow tD (4 * 63 * pow2 5 + 2 * 63) % prime384);
+    (==) {assert_by_tactic (4 * 63 * pow2 5 == 63 * (4 * pow2 5)) canon}
+    toDomain_ (pow tD (63 * (pow2 2 * pow2 5) + 2 * 63) % prime384);
+    (==) {pow2_plus 2 5}
+    toDomain_ (pow tD (63 * (pow2 7 + 2)) % prime384);};
+
+  let pow2_11 = pow2 11 in 
+  
+  calc (==) {
+    as_nat h12 t3;
+    (==) {}
+    toDomain_ (pow (pow tD (63 * (pow2 7 + 2)) % prime384) pow2_11  % prime384);
+    (==) {power_distributivity (pow tD (63 * (pow2 7 + 2))) pow2_11 prime384}
+    toDomain_ (pow (pow tD (63 * (pow2 7 + 2))) pow2_11  % prime384);
+    (==) {power_mult tD (63 * (pow2 7 + 2)) pow2_11}
+    toDomain_ (pow tD (63 * (pow2 7 + 2) *  pow2_11)  % prime384); }
+
+
+val lemma_exp1_4_2: t1D: nat -> t2D : nat -> t3D: nat -> prime384: pos  -> Lemma (    
+  toDomain_ ((pow t2D (pow2 6) * pow t3D (pow2 6) * t1D) % prime384 * ((pow t2D (pow2 6) * pow t3D (pow2 6) * t1D) % prime384) % prime384) == toDomain_ ((pow t2D (pow2 7) * pow t3D (pow2 7) * pow t1D 2) % prime384))
+  
+let lemma_exp1_4_2 t1D t2D t3D prime384 = 
+
+  calc (==) {
+    toDomain_ ((pow t2D (pow2 6) * pow t3D (pow2 6) * t1D) % prime384 * ((pow t2D (pow2 6) * pow t3D (pow2 6) * t1D) % prime384) % prime384);
+     (==) {lemma_mod_mul_distr (pow t2D (pow2 6) * pow t3D (pow2 6) * t1D) (pow t2D (pow2 6) * pow t3D (pow2 6) * t1D) prime384}
+     toDomain_ ((pow t2D (pow2 6) * pow t3D (pow2 6) * t1D) * (pow t2D (pow2 6) * pow t3D (pow2 6) * t1D) % prime384);
+     (==) {assert_by_tactic ((pow t2D (pow2 6) * pow t3D (pow2 6) * t1D) * (pow t2D (pow2 6) * pow t3D (pow2 6) * t1D) == 
+       (pow t2D (pow2 6) * pow t2D (pow2 6)) * (pow t3D (pow2 6) * pow t3D (pow2 6)) * (t1D * t1D)) canon}
+     toDomain_ ((pow t2D (pow2 6) * pow t2D (pow2 6)) * (pow t3D (pow2 6) * pow t3D (pow2 6)) * (t1D * t1D) % prime384);
+     (==) {pow_plus t2D (pow2 6) (pow2 6); pow_plus t3D (pow2 6) (pow2 6); power_one_2 t1D}
+     toDomain_ (pow t2D (2 * pow2 6) * pow t3D (2 * pow2 6) * (pow t1D 1 * pow t1D 1) % prime384);
+     (==) {pow2_double_sum 6; pow_plus t1D 1 1}
+     toDomain_ ((pow t2D (pow2 7) * pow t3D (pow2 7) * pow t1D 2) % prime384);}
+
+
+val lemma_exp1_5_2: tD: nat -> t1D: nat -> t2D : nat -> t3D: nat -> prime384: pos -> Lemma (
+  toDomain_ ((pow t2D (pow2 7) * pow t3D (pow2 7) * pow t1D 2 * tD % prime384) * (pow t2D (pow2 7) * pow t3D (pow2 7) * pow t1D 2 * tD % prime384) % prime384) ==
+    toDomain_ (((pow t2D (pow2 8)) * (pow t3D (pow2 8)) * (pow t1D 4) * (pow tD 2)) % prime384))
+
+
+let lemma_exp1_5_2 tD t1D t2D t3D prime384 = 
+  calc (==) {
+    toDomain_ ((pow t2D (pow2 7) * pow t3D (pow2 7) * pow t1D 2 * tD % prime384) * (pow t2D (pow2 7) * pow t3D (pow2 7) * pow t1D 2 * tD % prime384) % prime384);
+     (==) {lemma_mod_mul_distr (pow t2D (pow2 7) * pow t3D (pow2 7) * pow t1D 2 * tD) (pow t2D (pow2 7) * pow t3D (pow2 7) * pow t1D 2 * tD) prime384}
+     toDomain_ ((pow t2D (pow2 7) * pow t3D (pow2 7) * pow t1D 2 * tD) * (pow t2D (pow2 7) * pow t3D (pow2 7) * pow t1D 2 * tD) % prime384);
+     (==) {assert_by_tactic (((pow t2D (pow2 7) * pow t3D (pow2 7) * pow t1D 2 * tD) * (pow t2D (pow2 7) * pow t3D (pow2 7) * pow t1D 2 * tD)) == (pow t2D (pow2 7) * pow t2D (pow2 7)) * (pow t3D (pow2 7) * pow t3D (pow2 7)) * (pow t1D 2 * pow t1D 2) * (tD * tD)) canon}
+     toDomain_ (((pow t2D (pow2 7) * pow t2D (pow2 7)) * (pow t3D (pow2 7) * pow t3D (pow2 7)) * (pow t1D 2 * pow t1D 2) * (tD * tD)) % prime384);
+     (==) {pow_plus t2D (pow2 7) (pow2 7); pow_plus t3D (pow2 7) (pow2 7); pow_plus t1D 2 2; power_one_2 tD}
+     toDomain_ (((pow t2D (2 * pow2 7)) * (pow t3D (2 * pow2 7)) * (pow t1D 4) * (pow tD 1 * pow tD 1)) % prime384);
+     (==) {pow2_double_sum 7; pow_plus tD 1 1}
+     toDomain_ (((pow t2D (pow2 8)) * (pow t3D (pow2 8)) * (pow t1D 4) * (pow tD 2)) % prime384);}
+
+
+#set-options "--z3rlimit 300 --ifuel 0 --fuel 0"
+
+val exponent1: t: felem P384 -> t1: felem P384 -> t2: felem P384 -> t3: felem P384 -> t4: felem P384 ->  Stack unit 
+  (requires fun h -> live h t /\ live h t1 /\ live h t2 /\ live h t3 /\ live h t4 /\
+    LowStar.Monotonic.Buffer.all_disjoint [loc t; loc t1; loc t2; loc t3; loc t4] /\
+    as_nat h t < prime384 /\ as_nat h t1 < prime384 /\ as_nat h t2 < prime384 /\ as_nat h t3 < prime384)
+  (ensures fun h0 _ h1 -> True)
+
+
+let exponent1 t t1 t2 t3 t4 = 
+    let h0 = ST.get() in 
+  montgomery_multiplication_buffer_dh #P384 t2 t3 t2;
+    let h1 = ST.get() in 
 (* x30     = m(n_sq(x24 , 6) , _111111) *)
   fsquarePowN_dh #P384 (size 6) t2 ;
+    let h2 = ST.get() in 
   montgomery_multiplication_buffer_dh #P384 t2 t1 t1;  
+    let h3 = ST.get() in 
 (* t1 = x30 *)
-
 
 (* x31     = m(sq(x30), t) *)
   montgomery_square_buffer_dh #P384 t1 t2;
+    let h4 = ST.get() in 
   (* fsquarePowN_dh #P384 (size 29) t2 ; *)
   montgomery_multiplication_buffer_dh #P384 t2 t t2;
+    let h5 = ST.get() in 
 (* t2 = x31 *)
-
 
  (* x32     = m(sq(x31), t)  *)
   montgomery_square_buffer_dh #P384 t2 t3;
+    let h6 = ST.get() in 
   (* fsquarePowN_dh #P384 (size 30) t3 ; *)
   montgomery_multiplication_buffer_dh #P384 t t3 t3;
 (* t3 = x32*)
-
-
-
 
 (* x63     = m(n_sq(x32, 31) , x31) *)
   montgomery_square_buffer_dh #P384 t3 t4;
@@ -116,11 +308,69 @@ let exponent_p384 t result tempBuffer =
   montgomery_multiplication_buffer_dh #P384 t4 t2 t4;
 (* t4 = x63 *)
 
+   let tD = fromDomain_ (as_nat h0 t) in 
+   let t1D = fromDomain_ (as_nat h0 t1) in 
+   let t2D = fromDomain_ (as_nat h0 t2) in 
+   let t3D = fromDomain_ (as_nat h0 t3) in 
 
+   assert(as_nat h1 t2 = toDomain_ (t2D * t3D % prime384));
+   assert(as_nat h2 t2 = toDomain_ (pow (t2D * t3D % prime384) (pow2 6) % prime384));
+   assert(as_nat h3 t1 = toDomain_ (pow (t2D * t3D % prime384) (pow2 6) % prime384 * t1D % prime384));
+
+   calc(==) {
+     as_nat h2 t2;
+     (==) {}
+     toDomain_ (pow (t2D * t3D % prime384) (pow2 6) % prime384);
+     (==) {power_distributivity (t2D * t3D) (pow2 6) prime384}
+     toDomain_ (pow (t2D * t3D) (pow2 6) % prime384);
+     (==) {power_distributivity_2 t2D t3D (pow2 6)}
+     toDomain_ (pow t2D (pow2 6) * pow t3D (pow2 6) % prime384); };
+
+   calc (==) {
+     as_nat h3 t1;
+     (==) {}
+     toDomain_ (pow t2D (pow2 6) * pow t3D (pow2 6) % prime384 * t1D % prime384);
+     (==) {lemma_mod_mul_distr_l (pow t2D (pow2 6) * pow t3D (pow2 6)) t1D prime384}
+     toDomain_ (pow t2D (pow2 6) * pow t3D (pow2 6) * t1D % prime384);};
+
+   calc (==) {
+     as_nat h4 t2;
+     (==) {}
+     toDomain_ ((pow t2D (pow2 6) * pow t3D (pow2 6) * t1D) % prime384 * ((pow t2D (pow2 6) * pow t3D (pow2 6) * t1D) % prime384) % prime384);
+     (==) {lemma_exp1_4_2 t1D t2D t3D prime384}
+     toDomain_ ((pow t2D (pow2 7) * pow t3D (pow2 7) * pow t1D 2) % prime384);};
+
+   calc (==) {
+     as_nat h5 t2;
+     (==) {}
+     toDomain_ (((pow t2D (pow2 7) * pow t3D (pow2 7) * pow t1D 2) % prime384) * tD % prime384);
+     (==) {lemma_mod_mul_distr_l (pow t2D (pow2 7) * pow t3D (pow2 7) * pow t1D 2) tD prime384}
+     toDomain_ (pow t2D (pow2 7) * pow t3D (pow2 7) * pow t1D 2 * tD % prime384);};
+
+   calc (==) {
+     as_nat h6 t3;
+     (==) {}
+     toDomain_ ((pow t2D (pow2 7) * pow t3D (pow2 7) * pow t1D 2 * tD % prime384) * (pow t2D (pow2 7) * pow t3D (pow2 7) * pow t1D 2 * tD % prime384) % prime384);
+     (==) {lemma_exp1_5_2 tD t1D t2D t3D prime384}
+     toDomain_ (((pow t2D (pow2 8)) * (pow t3D (pow2 8)) * (pow t1D 4) * (pow tD 2)) % prime384);};
+
+
+   admit()
+
+
+
+val exponent2: t0: felem P384  -> t3: felem P384 -> t4: felem P384 -> t5: felem P384 -> Stack unit 
+  (requires fun h ->  live h t3 /\ live h t4 /\
+    LowStar.Monotonic.Buffer.all_disjoint [ loc t3; loc t4])
+  (ensures fun h0 _ h1 -> True)
+
+
+let exponent2 t0 t3 t4 t5  = 
 
 (* x126    = m(n_sq(x63, 63) , x63) *)
   montgomery_square_buffer_dh #P384 t4 t5;
-  fsquarePowN_dh #P384 (size 62) t5 ;
+  fsquarePowN_dh #P384 (size 62) t5;
+
   montgomery_multiplication_buffer_dh #P384 t4 t5 t4;  
 (* t4 = x126*)
 
@@ -140,10 +390,18 @@ let exponent_p384 t result tempBuffer =
 
 (* i0 = m(n_sq(x255, 33), x32) *)
   fsquarePowN_dh #P384 (size 33) t4 ;
-  montgomery_multiplication_buffer_dh #P384 t4 t3 t4;
+  montgomery_multiplication_buffer_dh #P384 t4 t3 t4
 (*t4 = i0 *)
 
 
+val exponent3: t: felem P384 -> t1: felem P384 -> t4: felem P384 -> result: felem P384 -> Stack unit 
+  (requires fun h -> live h t /\ live h t1 /\ live h t4 /\ live h result /\
+    LowStar.Monotonic.Buffer.all_disjoint [loc t; loc t1; loc t4] /\
+    as_nat h t < prime384 /\ as_nat h t1 < prime384 /\ as_nat h t4 < prime384)
+  (ensures fun h0 _ h1 -> modifies (loc t1 |+| loc t4 |+| loc result) h0 h1)
+
+
+let exponent3 t t1 t4 result = 
 (* i1 = m(n_sq(i0, 94), x30) *)
   fsquarePowN_dh #P384 (size 94) t4 ;
   montgomery_multiplication_buffer_dh #P384 t4 t1 t4;
@@ -154,3 +412,31 @@ let exponent_p384 t result tempBuffer =
 
 (* r = m(t, i397) *)
   montgomery_multiplication_buffer_dh #P384 t4 t result
+
+
+val exponent_p384: a: felem P384 -> result: felem P384 -> 
+  tempBuffer: lbuffer uint64 (getCoordinateLenU P384 *. 8ul) -> Stack unit
+  (requires fun h -> live h a /\ live h tempBuffer /\ live h result /\ disjoint tempBuffer result /\ 
+    disjoint a tempBuffer /\ as_nat  h a < getPrime P384)
+  (ensures fun h0 _ h1 -> modifies (loc result |+| loc tempBuffer) h0 h1 /\ (
+    let k = fromDomain #P384 (as_nat h0 a) in True ))(*
+    as_nat P384 h1 result =  toDomain #P384 (pow k (prime384 - 2) % prime256) *) 
+
+
+let exponent_p384 t result tempBuffer = 
+  let h0 = ST.get () in 
+
+  let t0 = sub tempBuffer (size 0) (size 6) in 
+
+  let t1 = sub tempBuffer (size 6) (size 6) in 
+  let t2 = sub tempBuffer (size 12) (size 6) in 
+  let t3 = sub tempBuffer (size 18) (size 6) in 
+  let t4 = sub tempBuffer (size 24) (size 6) in 
+  let t5 = sub tempBuffer (size 30) (size 6) in 
+
+  exponent0 t t0 t1 t2 t3;
+  exponent1 t t1 t2 t3 t4;
+  exponent2 t0 t3 t4 t5;
+  exponent3 t t1 t4 result
+
+
